massive update

src/MemoryOps.v
@@ -1,6 +1,10 @@
-Require Addressing Common Condition CallStack Memory Instruction.
+From RecordUpdate Require Import RecordSet.
 
-Import Addressing ZArith ZMod Common Condition CallStack MemoryBase Memory Instruction Pages List ListNotations.
+Require Addressing Common Condition CallStack Error Memory Instruction.
+
+Import Addressing ZArith ZMod Common Condition CallStack MemoryBase Memory Instruction Pages List ListNotations Error String.
+Import RecordSetNotations.
+Open Scope error_monad_scope.
 
 Inductive endianness := LittleEndian | BigEndian.
 
@@ -11,9 +15,8 @@ Inductive loc : Set :=
 | LocStackAddress: stack_address -> loc
 | LocCodeAddr: code_address -> loc
 | LocConstAddr: const_address ->  loc
-| LocHeapAddr: page_id -> mem_address -> loc
-| LocAuxHeapAddr: page_id -> mem_address ->  loc.
-
+(* | LocHeapVariantAddr: page_id -> mem_address -> loc *)
+.
 
 Section GPR.
   (** Fetching value from general purpose register. *)
@@ -117,8 +120,38 @@ Section GPR.
         (mk_regs r1 r2 r3 r4 r5 r6 r7 r8 r9 r10 r11 r12 r13 r14 pv)
   .
 
+
+Definition do_store_gpr (r: regs_state) (rn: reg_name) (pv: primitive_value) : res regs_state :=
+  match rn with
+    | R0 => Error (msg "Can not store register R0 is read only")
+  | R1 => OK (r <| gprs_r1 := pv|>)
+  | R2 => OK (r <| gprs_r2 := pv|>)
+  | R3 => OK (r <| gprs_r3 := pv|>)
+  | R4 => OK (r <| gprs_r4 := pv|>)
+  | R5 => OK (r <| gprs_r5 := pv|>)
+  | R6 => OK (r <| gprs_r6 := pv|>)
+  | R7 => OK (r <| gprs_r7 := pv|>)
+  | R8 => OK (r <| gprs_r8 := pv|>)
+  | R9 => OK (r <| gprs_r9 := pv|>)
+  | R10 => OK (r <| gprs_r10 := pv|>)
+  | R11 => OK (r <| gprs_r11 := pv|>)
+  | R12 => OK (r <| gprs_r12 := pv|>)
+  | R13 => OK (r <| gprs_r13 := pv|>)
+  | R14 => OK (r <| gprs_r14 := pv|>)
+  | R15 => OK (r <| gprs_r15 := pv|>)
+  end.
+                                                          
+  Definition store_gpr_correct:
+    forall regs rn pv regs',
+    store_gpr regs rn pv regs' ->
+    do_store_gpr regs rn pv = OK regs'.
+  Proof. destruct 1; constructor. Qed.
+  
+    
 End GPR.
 
+
+  
 Section Addressing.
 
   Inductive reg_rel addr_bits : regs_state -> reg_name -> int_mod addr_bits -> int_mod addr_bits -> Prop :=
@@ -129,6 +162,26 @@ Section Addressing.
       base + ofs = (abs, OF_ignored) ->
       reg_rel addr_bits regs reg ofs abs.
 
+  Definition do_reg_rel {addr_bits} (rs: regs_state) (r: reg_name) (ofs: int_mod addr_bits) :  res( int_mod addr_bits) :=
+      match fetch_gpr rs r with
+       | IntValue reg_val =>
+           OK (add_wrap _ (resize _ addr_bits reg_val) ofs)
+      |_ => Error (msg "Expected a non-pointer value in register")
+      end.
+
+  Theorem reg_rel_spec :
+    forall addr_bits rs r ofs abs,
+      @reg_rel addr_bits rs r ofs abs ->
+      @do_reg_rel addr_bits rs r ofs = OK abs.
+  Proof.
+    intros addr_bits rs r ofs abs H.
+    inv H.
+    inv H2.
+    inv H1.
+    unfold do_reg_rel, resize, add_wrap, uadd_overflow, as_unsigned in *.
+    rewrite H0; auto.
+  Qed.
+  
   Definition reg_rel_code : regs_state -> reg_name -> u16 -> code_address -> Prop
     := reg_rel code_address_bits.
 
@@ -164,20 +217,22 @@ Section Addressing.
   | rslv_stack_rel_aux: forall ef regs reg offset_imm dlt_sp sp_rel OF_ignore,
       let base := sp_get ef in
       sp_delta_abs regs reg offset_imm dlt_sp ->
-      (sp_rel, OF_ignore) = usub_overflow _ base dlt_sp->
+      (sp_rel, OF_ignore) = base - dlt_sp->
       loc_stack_io ef regs (RelSP reg offset_imm) (LocStackAddress sp_rel)
+                   
   | rslv_stack_abs_aux: forall ef regs reg imm abs,
       reg_rel_stack regs reg imm abs ->
-      loc_stack_io ef regs (Absolute reg imm) (LocStackAddress imm).
+      loc_stack_io ef regs (Absolute reg imm) (LocStackAddress abs).
 
+(* FIXME of should not be ignored*)
   Inductive loc_stack_in_only: callstack -> regs_state -> stack_in_only -> loc -> Prop :=
   | rslv_stack_gpop_aux: forall ef regs reg ofs dlt_sp new_sp OF_ignore,
       let sp := sp_get ef in
       sp_delta_abs regs reg ofs dlt_sp ->
-      (new_sp, OF_ignore) = usub_overflow _ sp dlt_sp ->
+      (new_sp, OF_ignore) = sp - dlt_sp ->
       loc_stack_in_only ef regs (RelSpPop reg ofs) (LocStackAddress new_sp)
   .
-
+(* FIXME of should not be ignored*)
   Inductive loc_stack_out_only: callstack -> regs_state -> stack_out_only -> loc -> Prop :=
   | rslv_stack_gpush_aux: forall ef regs reg ofs dlt_sp new_sp OF_ignore,
       let sp := sp_get ef in
@@ -210,6 +265,99 @@ Section Addressing.
       resolve ef regs (AnyConst arg) loc
   .
 
+                      
+  Definition do_resolve (xstack: callstack) (rs:regs_state) (a:any) : res loc :=
+    match a with
+    | AnyReg (Reg r) => OK (LocReg r)
+    | AnyImm (Imm i) => OK (LocImm i)
+    | AnyStack (StackAnyIO (Absolute r ofs)) =>
+        do abs <- do_reg_rel rs r ofs ;
+        OK (LocStackAddress abs)
+    | AnyStack (StackAnyIO (RelSP r ofs)) =>  
+        do sp_ofs <- do_reg_rel rs r ofs ;
+        let abs := sub_wrap _ (sp_get xstack) sp_ofs in
+        OK (LocStackAddress abs)
+    | AnyStack (StackAnyIn (RelSpPop r ofs)) =>
+        do sp_ofs <- do_reg_rel rs r ofs ;
+        let abs := sub_wrap _ (sp_get xstack) sp_ofs in
+        OK (LocStackAddress abs)
+                  
+    | AnyStack (StackAnyOut (RelSpPush r ofs)) =>
+        do sp_ofs <- do_reg_rel rs r ofs ;
+        let abs := add_wrap _ (sp_get xstack) sp_ofs in
+        OK (LocStackAddress abs)
+    | AnyCode (CodeAddr r ofs) =>
+        do abs <- do_reg_rel rs r ofs ;
+        OK (LocCodeAddr abs)
+    | AnyConst (ConstAddr r ofs) => 
+        do abs <- do_reg_rel rs r ofs ;
+        OK (LocConstAddr abs)
+    end .
+
+  Theorem do_resolve_correct:
+    forall xstack rs a res,
+      resolve xstack rs a res ->
+      do_resolve xstack rs a = OK res.
+  Proof.
+{
+  intros xstack rs [] res; inversion_clear 1; subst; simpl.
+  - destruct r;  auto; inversion_clear H0; auto.
+  - destruct i;  auto; inversion_clear H0; auto.
+  - inversion_clear H0.
+    + inv H.
+      exploit (reg_rel_spec (address_bits stack_page_params)).
+      * econstructor; eauto.
+      * intro H'.
+        simpl in *. rewrite H'.
+        simpl.
+        inv H3.
+        inv H1.
+        repeat f_equal.
+    +  inv H.
+       unfold do_reg_rel.
+       rewrite H0.
+       unfold add_wrap, uadd_overflow in *.
+       inv H2.
+       inv H1.
+       simpl.
+       repeat f_equal.
+  - inv H0.
+    inv H.
+    inv H0.
+    inv H2.
+    inv H3.
+    unfold do_reg_rel.
+    rewrite H4.
+    unfold add_wrap, uadd_overflow, sub_wrap, usub_overflow in *.
+    simpl.
+    inv H1.
+    reflexivity.
+  - inv H0.   
+    inv H.   
+    inv H1.
+    inv H3.
+    inv H2.
+    unfold do_reg_rel.
+    rewrite H0.
+    reflexivity.
+  - inv H0.
+    inv H.
+    inv H2.
+    inv H1.
+    unfold do_reg_rel.
+    rewrite H0.
+    reflexivity.
+  - inv H0.
+    inv H.
+    inv H2.
+    inv H1.
+    unfold do_reg_rel.
+    rewrite H0.
+    reflexivity.
+}
+  Qed.
+
+  
   Inductive resolve_effect__in: in_any -> callstack -> callstack -> Prop :=
   | rslv_stack_in_effect: forall ef ef' regs sp' reg ofs arg,
       loc_stack_in_only ef regs  arg (LocStackAddress sp') ->
@@ -250,38 +398,10 @@ Section FetchStore.
 
   Context {instruction: Type} (inv: instruction).
  
-  Let pages := pages instruction_invalid.
+  Let memory := Pages.memory instruction_invalid.
   Inductive fetch_result : Set :=
   | FetchIns (ins :instruction_predicated)
   | FetchPV (pv: primitive_value) .
-
-  (* Address resolution *)
-  Inductive fetch_loc: regs_state -> callstack -> pages -> loc -> fetch_result -> Prop :=
-  | fetch_reg:
-    forall regs ef mm reg_name,
-      fetch_loc regs ef mm (LocReg reg_name) (FetchPV (fetch_gpr regs reg_name))
-
-  | fetch_imm:
-    forall regs ef mm imm imm',
-      imm' = resize _ word_bits imm ->
-      fetch_loc regs ef mm (LocImm imm) (FetchPV (IntValue imm'))
-
-  | fetch_stackaddr:
-    forall regs ef ps stackpage addr value,
-      active_stackpage _ ps ef (StackPage _ stackpage) ->
-      load_result _ addr stackpage value ->
-      fetch_loc regs ef ps (LocStackAddress addr) (FetchPV value)
-  | fetch_codeaddr:
-    forall regs ef ps codepage addr ins,
-      active_codepage _ ps ef (CodePage _ codepage) ->
-      load_result _ addr codepage ins ->
-      fetch_loc regs ef ps (LocCodeAddr addr) (FetchIns ins)
-  | fetch_constaddr:
-    forall regs ef ps constpage addr value,
-      active_codepage _ ps ef (ConstPage _ constpage) ->
-      load_result _ addr constpage value ->
-      fetch_loc regs ef ps (LocConstAddr addr) (FetchPV (IntValue value))
-  .
 
   Definition load_word (e: endianness) (mem:data_page) (addr:mem_address) :option word :=
     match load_multicell data_page_params addr bytes_in_word mem with
@@ -316,12 +436,47 @@ Section FetchStore.
       load_slice_word e mem addr = Some res ->
       load_slice_result e mem addr res.
   
-  Inductive fetch_instr : regs_state -> callstack -> pages -> instruction_predicated -> Prop :=
+  (* Address resolution *)
+  Inductive fetch_loc: regs_state -> callstack -> memory -> loc -> fetch_result -> Prop :=
+  | fetch_reg:
+    forall regs ef mm reg_name,
+      fetch_loc regs ef mm (LocReg reg_name) (FetchPV (fetch_gpr regs reg_name))
+
+  | fetch_imm:
+    forall regs ef mm imm imm',
+      imm' = resize _ word_bits imm ->
+      fetch_loc regs ef mm (LocImm imm) (FetchPV (IntValue imm'))
+
+  | fetch_stackaddr:
+    forall regs ef ps stackpage addr value,
+      active_stackpage _ ps ef (StackPage _ stackpage) ->
+      MemoryBase.load_result _ addr stackpage value ->
+      fetch_loc regs ef ps (LocStackAddress addr) (FetchPV value)
+  | fetch_codeaddr:
+    forall regs ef ps codepage addr ins,
+      active_codepage _ ps ef (CodePage _ codepage) ->
+      MemoryBase.load_result _ addr codepage ins ->
+      fetch_loc regs ef ps (LocCodeAddr addr) (FetchIns ins)
+  | fetch_constaddr:
+    forall regs ef ps constpage addr value,
+      active_codepage _ ps ef (ConstPage _ constpage) ->
+      MemoryBase.load_result _ addr constpage value ->
+      fetch_loc regs ef ps (LocConstAddr addr) (FetchPV (IntValue value))
+
+                
+  (*   forall regs ef ps dp pid addr value, *)
+  (*     page_has_id _ ps pid (DataPage _ dp) -> *)
+  (*     load_result BigEndian dp addr value -> *)
+  (*     fetch_loc regs ef ps (LocHeapVariantAddr pid addr) (FetchPV (IntValue value)) *)
+  .
+
+  
+  Inductive fetch_instr : regs_state -> callstack -> memory -> instruction_predicated -> Prop :=
   | fi_fetch: forall regs ef mm ins,
       fetch_loc regs ef mm (LocCodeAddr (pc_get ef)) (FetchIns ins) ->
       fetch_instr regs ef mm ins.
 
-  Inductive store_loc: regs_state -> callstack -> pages -> primitive_value -> loc -> (regs_state * pages) -> Prop :=
+  Inductive store_loc: regs_state -> callstack -> memory -> primitive_value -> loc -> (regs_state * memory) -> Prop :=
   | store_reg:
     forall regs regs' ef mm reg_name value,
       store_gpr regs reg_name value regs' ->
@@ -350,57 +505,57 @@ Section FetchStore.
       store_word e page addr val = Some page' ->
       store_word_result e page addr val page'.
   
-  Inductive resolve_load: callstack -> (regs_state * pages) -> any -> primitive_value -> Prop :=
+  Inductive resolve_load: callstack -> (regs_state * memory) -> any -> primitive_value -> Prop :=
   | rf_resfetch_pv: forall ef mm regs arg loc res,
       resolve ef regs arg loc ->
       fetch_loc regs ef mm loc (FetchPV res) ->
       resolve_load ef (regs , mm) arg res.
 
-  Inductive resolve_loads: callstack -> (regs_state * pages)
+  Inductive resolve_loads: callstack -> (regs_state * memory)
                             -> list (in_any * primitive_value) 
                             -> Prop :=
   | rsl_nil: forall ef s ,
       resolve_loads ef s nil
                     
-  | rsl_cons: forall ef regs pages (arg:in_any) pv (tail: list (in_any*primitive_value)),
-      resolve_loads ef (regs, pages) tail ->
-      resolve_load  ef (regs, pages ) (in_any_incl arg) pv ->
-      resolve_loads ef (regs, pages ) ((arg,pv)::tail).
+  | rsl_cons: forall ef regs memory (arg:in_any) pv (tail: list (in_any*primitive_value)),
+      resolve_loads ef (regs, memory) tail ->
+      resolve_load  ef (regs, memory ) (in_any_incl arg) pv ->
+      resolve_loads ef (regs, memory ) ((arg,pv)::tail).
 
   
-  Inductive resolve_load_word: callstack -> regs_state * pages -> any -> word -> Prop :=
+  Inductive resolve_load_word: callstack -> regs_state * memory -> any -> word -> Prop :=
   | rf_resfetch_w: forall ef s arg res,
       resolve_load ef s arg (IntValue res) ->
       resolve_load_word ef s arg res.
 
-  Inductive resolve_load_words: callstack -> (regs_state * pages)
+  Inductive resolve_load_words: callstack -> (regs_state * memory)
                             -> list (in_any * word) 
                             -> Prop :=
   | rslw_nil: forall ef s ,
       resolve_load_words ef s nil
                     
-  | rslw_cons: forall ef regs pages (arg:in_any) pv (tail: list (in_any*word)),
-      resolve_load_words ef (regs, pages) tail ->
-      resolve_load_word ef (regs, pages ) (in_any_incl arg) pv ->
-      resolve_load_words ef (regs, pages ) ((arg,pv)::tail).
+  | rslw_cons: forall ef regs memory (arg:in_any) pv (tail: list (in_any*word)),
+      resolve_load_words ef (regs, memory) tail ->
+      resolve_load_word ef (regs, memory ) (in_any_incl arg) pv ->
+      resolve_load_words ef (regs, memory ) ((arg,pv)::tail).
 
-  Inductive resolve_store: callstack -> (regs_state * pages)
-                           -> out_any -> primitive_value -> regs_state * pages
+  Inductive resolve_store: callstack -> (regs_state * memory)
+                           -> out_any -> primitive_value -> regs_state * memory
                            -> Prop :=
   | rs_resstore: forall ef mm regs arg loc_out pv regs' mm',
       resolve ef regs (out_any_incl arg) loc_out ->
       store_loc regs ef mm pv loc_out (regs', mm') ->
       resolve_store ef (regs, mm) arg pv (regs', mm').
 
-  Inductive resolve_stores: callstack -> (regs_state * pages)
-                            -> list (out_any * primitive_value) -> (regs_state * pages)
+  Inductive resolve_stores: callstack -> (regs_state * memory)
+                            -> list (out_any * primitive_value) -> (regs_state * memory)
                             -> Prop :=
   | rss_nil: forall ef s ,
       resolve_stores ef s nil s
-  | rss_cons: forall ef regs pages regs' pages' regs'' pages'' out pv tail,
-      resolve_stores ef (regs', pages') tail (regs'', pages'') ->
-      resolve_store ef (regs,pages) out pv (regs', pages') ->
-      resolve_stores ef (regs, pages) (cons (out,pv) tail)  (regs'', pages'').
+  | rss_cons: forall ef regs memory regs' memory' regs'' memory'' out pv tail,
+      resolve_stores ef (regs', memory') tail (regs'', memory'') ->
+      resolve_store ef (regs,memory) out pv (regs', memory') ->
+      resolve_stores ef (regs, memory) (cons (out,pv) tail)  (regs'', memory'').
 
   Record fqa_storage := mk_fqa_storage {
                         k_shard: shard_id;
@@ -432,3 +587,4 @@ Section FetchStore.
       storage_write d (mk_fqa_key sk k) w depot'.
 
 End FetchStore.
+ 
