src/Event.v
@@ -1,0 +1,33 @@
+Require Memory External.
+Import Common Memory External.
+
+
+
+(* For later: probably these structures can be redesigned so that *)
+
+Record event := {
+    ev_shard_id: shard_id;
+    ev_is_first: bool;
+    ev_tx_number_in_block: tx_num;
+    ev_address: contract_address;
+    ev_key: word;
+    ev_value: word;
+}.
+
+
+Record precompile_query := {
+    q_timestamp: timestamp;
+    q_tx_number_in_block: tx_num;
+    q_shard_id: shard_id;
+    q_contract_address: contract_address;
+    q_key: word;
+    q_is_service: bool; (* is first message? *)
+}.
+
+Inductive query :=
+  (* | StorageQuery : query *)
+  | EventQuery : event -> query
+  (* | L1MsgQuery : event -> query *)
+  | PrecompileQuery : precompile_query -> query.
+
+         
