src/External.v
@@ -1,0 +1,7 @@
+Require Common.
+
+Import Common.
+
+
+Definition timestamp := nat.
+Definition tx_num := u16.
