src/sem/Context.v
@@ -8,184 +8,162 @@ Import Addressing ABI Bool Common Condition Ergs CallStack Memory MemoryOps Inst
 Inductive step: instruction -> smallstep :=
 
 | step_ContextThis:
-  forall gs flags pages xstack context_u128 regs (out_arg:out_reg) this_addr new_regs new_pages,
+  forall flags pages xstack regs (out_arg:out_reg) this_addr new_regs new_pages s1 s2,
     resolve_store xstack (regs,pages)
       out_arg (IntValue this_addr) (new_regs, new_pages) ->
     this_addr = resize contract_address_bits word_bits (topmost_extframe xstack).(ecf_this_address) ->
-    
-    step (OpContextThis out_arg)
-         {|
-           gs_regs         := regs;
-           gs_pages        := pages;
-           
-           gs_callstack    := xstack;
-           gs_flags        := flags;
-           
-           gs_context_u128 := context_u128;
-           gs_global       := gs;
-         |}
-         {|
-           gs_regs         := new_regs;
-           gs_pages        := new_pages;
 
+    step_xstate
+      {|
+        gs_regs         := regs;
+        gs_pages        := pages;
+        
+        gs_callstack    := xstack;
+        gs_flags        := flags;
+        
+      |}
+      {|
+        gs_regs         := new_regs;
+        gs_pages        := new_pages;
 
-           gs_callstack    := xstack;
-           gs_flags        := flags;
-           
-           gs_context_u128 := context_u128;
-           gs_global       := gs;
-         |}
+        
+        gs_callstack    := xstack;
+        gs_flags        := flags;
+      |} s1 s2 ->
+    step (OpContextThis out_arg) s1 s2
+
 | step_ContextCaller:
-  forall gs flags  pages xstack context_u128 regs (out_arg:out_reg) sender_addr new_regs new_pages,
+  forall flags pages xstack regs (out_arg:out_reg) sender_addr new_regs new_pages s1 s2,
     resolve_store xstack (regs,pages)
       out_arg (IntValue sender_addr)
       (new_regs, new_pages) ->
-    sender_addr = resize contract_address_bits word_bits (topmost_extframe xstack).(ecf_msg_sender) ->
     
-    step (OpContextCaller out_arg)
-         {|
-           gs_regs         := regs;
-           gs_pages        := pages;
-           
-           gs_callstack    := xstack;
-           gs_flags        := flags;
-           
-           gs_context_u128 := context_u128;
-           gs_global       := gs;
-         |}
-         {|
-           gs_regs         := new_regs;
-           gs_pages        := new_pages;
+    sender_addr = resize contract_address_bits word_bits (topmost_extframe xstack).(ecf_msg_sender) ->
 
+    step_xstate
+      {|
+        gs_regs         := regs;
+        gs_pages        := pages;
+        
+        gs_callstack    := xstack;
+        gs_flags        := flags;
+        
+      |}
+      {|
+        gs_regs         := new_regs;
+        gs_pages        := new_pages;
 
-           gs_callstack    := xstack;
-           gs_flags        := flags;
-           
-           gs_context_u128 := context_u128;
-           gs_global       := gs;
-         |}
+        
+        gs_callstack    := xstack;
+        gs_flags        := flags;
+      |} s1 s2 ->
+    step (OpContextCaller out_arg) s1 s2
+         
 | step_ContextCodeAddress:
-  forall gs flags  pages xstack context_u128 regs (out:out_reg) code_addr new_regs new_pages,
+  forall flags  pages xstack regs (out:out_reg) code_addr new_regs new_pages s1 s2,
     resolve_store xstack (regs,pages)
       out (IntValue code_addr) (new_regs, new_pages) ->
     
     code_addr = resize code_address_bits word_bits (pc_get xstack) -> 
     
-    step (OpContextCaller out)
-         {|
-           gs_regs         := regs;
-           gs_pages        := pages;
-           
-           gs_callstack    := xstack;
-           gs_flags        := flags;
-           
-           gs_context_u128 := context_u128;
-           gs_global       := gs;
-         |}
-         {|
-           gs_regs         := new_regs;
-           gs_pages        := new_pages;
+    step_xstate
+      {|
+        gs_regs         := regs;
+        gs_pages        := pages;
+        
+        gs_callstack    := xstack;
+        gs_flags        := flags;
+        
+      |}
+      {|
+        gs_regs         := new_regs;
+        gs_pages        := new_pages;
 
-
-           gs_callstack    := xstack;
-           gs_flags        := flags;
-           
-           gs_context_u128 := context_u128;
-           gs_global       := gs;
-         |}
+        
+        gs_callstack    := xstack;
+        gs_flags        := flags;
+      |} s1 s2 ->
+    step (OpContextCodeAddress out) s1 s2
 | step_ContextErgsLeft:
-  forall gs flags  pages xstack context_u128 regs (out_arg:out_reg) balance new_regs new_pages,
+  forall flags  pages xstack regs (out_arg:out_reg) balance new_regs new_pages s1 s2,
     resolve_store xstack (regs,pages)
       out_arg (IntValue balance) (new_regs, new_pages) ->
     
     balance = resize _ word_bits (topmost_extframe xstack).(ecf_common).(cf_ergs_remaining) ->
-    
-    step (OpContextErgsLeft out_arg)
-         {|
-           gs_regs         := regs;
-           gs_pages        := pages;
-           
-           gs_callstack    := xstack;
-           gs_flags        := flags;
-           
-           gs_context_u128 := context_u128;
-           gs_global       := gs;
-         |}
-         {|
-           gs_regs         := new_regs;
-           gs_pages        := new_pages;
+     step_xstate
+      {|
+        gs_regs         := regs;
+        gs_pages        := pages;
+        
+        gs_callstack    := xstack;
+        gs_flags        := flags;
+        
+      |}
+      {|
+        gs_regs         := new_regs;
+        gs_pages        := new_pages;
 
+        
+        gs_callstack    := xstack;
+        gs_flags        := flags;
+      |} s1 s2 ->
 
-           gs_callstack    := xstack;
-           gs_flags        := flags;
-           
-           gs_context_u128 := context_u128;
-           gs_global       := gs;
-         |}
+    step (OpContextErgsLeft out_arg) s1 s2
+         
          
 | step_ContextSP:
-  forall gs flags  pages xstack context_u128 regs (out_arg:out_reg) sp new_regs new_pages,
+  forall flags  pages xstack regs (out_arg:out_reg) sp new_regs new_pages s1 s2,
     resolve_store xstack (regs,pages)
       out_arg (IntValue sp) (new_regs, new_pages) ->
     
     sp = resize _ word_bits (sp_get xstack) ->
     
-    step (OpContextSp out_arg)
-         {|
-           gs_regs         := regs;
-           gs_pages        := pages;
-           
-           gs_callstack    := xstack;
-           gs_flags        := flags;
-           
-           gs_context_u128 := context_u128;
-           gs_global       := gs;
-         |}
-         {|
-           gs_regs         := new_regs;
-           gs_pages        := new_pages;
+     step_xstate
+      {|
+        gs_regs         := regs;
+        gs_pages        := pages;
+        
+        gs_callstack    := xstack;
+        gs_flags        := flags;
+        
+      |}
+      {|
+        gs_regs         := new_regs;
+        gs_pages        := new_pages;
 
-
-           gs_callstack    := xstack;
-           gs_flags        := flags;
-           
-           gs_context_u128 := context_u128;
-           gs_global       := gs;
-         |}
+        
+        gs_callstack    := xstack;
+        gs_flags        := flags;
+      |} s1 s2 ->
+    step (OpContextSp out_arg) s1 s2
          
 | step_ContextGetContextU128:
-  forall gs flags  pages xstack context_u128 regs (out_arg:out_reg) new_regs new_pages wcontext,
+  forall flags pages xstack regs (out_arg:out_reg) new_regs new_pages wcontext s1 s2,
     resolve_store xstack (regs,pages)
       out_arg (IntValue wcontext) (new_regs, new_pages) ->
 
-    wcontext = resize _ word_bits context_u128 ->  
+    wcontext = resize _ word_bits (gs_context_u128 s1) ->  
     
-    step (OpContextGetContextU128 out_arg)
-         {|
-           gs_regs         := regs;
-           gs_pages        := pages;
+     step_xstate
+      {|
+        gs_regs         := regs;
+        gs_pages        := pages;
+        
+        gs_callstack    := xstack;
+        gs_flags        := flags;
+        
+      |}
+      {|
+        gs_regs         := new_regs;
+        gs_pages        := new_pages;
 
-           
-           gs_callstack    := xstack;
-           gs_flags        := flags;
-           
-           gs_context_u128 := context_u128;
-           gs_global       := gs;
-         |}
-         {|
-           gs_regs         := new_regs;
-           gs_pages        := new_pages;
-
-           
-           gs_callstack    := xstack;
-           gs_flags        := flags;
-           
-           gs_context_u128 := context_u128;
-           gs_global       := gs;
-         |}
-         
+        
+        gs_callstack    := xstack;
+        gs_flags        := flags;
+      |} s1 s2 ->
+    step (OpContextGetContextU128 out_arg) s1 s2
 | step_ContextSetContextU128:
-  forall gs flags  pages xstack old_context_u128 regs (in_arg:in_reg) any_tag val new_context_u128,
+  forall gs pages xstack old_context_u128 regs (in_arg:in_reg) any_tag val new_context_u128 xstate,
     resolve_load xstack (regs,pages) in_arg (mk_pv any_tag val) ->
 
     new_context_u128 = resize word_bits 128 val ->
@@ -193,29 +171,21 @@ Inductive step: instruction -> smallstep :=
          {|
            gs_context_u128 := old_context_u128;
 
-           
-           gs_regs         := regs;
-           gs_pages        := pages;
-           gs_callstack    := xstack;
-           gs_flags        := flags;
-           
+
+           gs_xstate := xstate;
            gs_global       := gs;
          |}
          {|
            gs_context_u128 := new_context_u128;
 
            
-           gs_regs         := regs;
-           gs_pages        := pages;
-           gs_callstack    := xstack;
-           gs_flags        := flags;
-           
+           gs_xstate := xstate;
            gs_global       := gs;
          |}
 
 | step_ContextMeta:
-  forall gs flags  pages xstack context_u128 regs (out_arg:out_reg) new_regs new_pages meta_encoded
-    ergs_per_pubdata,
+  forall flags  pages xstack regs (out_arg:out_reg) new_regs new_pages meta_encoded
+    ergs_per_pubdata s1 s2,
     resolve_store xstack (regs,pages)
       out_arg (IntValue meta_encoded) (new_regs, new_pages) ->
 
@@ -231,84 +201,58 @@ Inductive step: instruction -> smallstep :=
                              code_shard_id := shard_code shards;
                            |} ->
     
-    step (OpContextMeta out_arg)
-         {|
-           gs_regs         := regs;
-           gs_pages        := pages;
+     step_xstate
+      {|
+        gs_regs         := regs;
+        gs_pages        := pages;
+        
+        gs_callstack    := xstack;
+        gs_flags        := flags;
+        
+      |}
+      {|
+        gs_regs         := new_regs;
+        gs_pages        := new_pages;
 
-           
-           gs_callstack    := xstack;
-           gs_flags        := flags;
-           
-           gs_context_u128 := context_u128;
-           gs_global       := gs;
-         |}
-         {|
-           gs_regs         := new_regs;
-           gs_pages        := new_pages;
-
-           
-           gs_callstack    := xstack;
-           gs_flags        := flags;
-           
-           gs_context_u128 := context_u128;
-           gs_global       := gs;
-         |}
+        
+        gs_callstack    := xstack;
+        gs_flags        := flags;
+      |} s1 s2 ->
+    step (OpContextMeta out_arg) s1 s2
 | step_ContextIncTx:
-  forall flags regs pages xstack context_u128 gs new_gs,
+  forall context_u128 gs new_gs xstate,
    global_state_increment_tx gs new_gs -> 
     step OpContextIncrementTxNumber
          {|
-           gs_regs         := regs;
-           gs_pages        := pages;
-
-           
-           gs_callstack    := xstack;
-           gs_flags        := flags;
+           gs_xstate       := xstate;
            
            gs_context_u128 := context_u128;
            gs_global       := gs;
          |}
          {|
-           gs_regs         := regs;
-           gs_pages        := pages;
-
-           
-           gs_callstack    := xstack;
-           gs_flags        := flags;
-           
+           gs_xstate       := xstate;
            gs_context_u128 := context_u128;
-           gs_global       := gs;
+           gs_global       := new_gs;
          |}
 | step_ContextSetErgsPerPubdata:
-  forall gs new_gs flags  pages xstack context_u128 regs (in_arg:in_reg) any_tag new_val (new_val_arg:in_reg),
+  forall gs new_gs pages context_u128 regs (in_arg:in_reg) any_tag new_val (new_val_arg:in_reg) xstate ,
 
-    resolve_load xstack (regs, pages) in_arg (mk_pv any_tag new_val) ->
+    resolve_load xstate.(gs_callstack) (regs, pages) in_arg (mk_pv any_tag new_val) ->
 
     let new_ergs := resize _ ergs_bits new_val in
     new_gs = gs <| gs_global ::= (fun s => s <| gs_current_ergs_per_pubdata_byte := new_ergs |> ) |> ->
                                  
     step (OpContextSetErgsPerPubdataByte new_val_arg)
          {|
-           gs_regs         := regs;
-           gs_pages        := pages;
-
-           
-           gs_callstack    := xstack;
-           gs_flags        := flags;
+           gs_xstate       := xstate;
            
            gs_context_u128 := context_u128;
            gs_global       := gs;
          |}
          {|
-           gs_regs         := regs;
-           gs_pages        := pages;
-
-           
-           gs_callstack    := xstack;
-           gs_flags        := flags;
-           
+           gs_xstate       := xstate;
            gs_context_u128 := context_u128;
-           gs_global       := gs;
+           gs_global       := new_gs;
          |}
-.
+
+.        
