src/sem/Div.v
@@ -7,24 +7,23 @@ Import Addressing Bool ZArith Common Condition Instruction CallStack Memory Memo
 Section Def.
   Local Coercion u256_of : Z >-> int_mod.
   Open Scope Z_scope.
-  Context (flags: flags_state) (regs: regs_state) (xstack: callstack) (pgs: pages).
+  Context (flags: flags_state) (regs: regs_state) (xstack: callstack) (pgs: memory).
 
-  Inductive step_div: instruction -> flags_state * regs_state * callstack * pages -> Prop :=
+  Inductive step_div: instruction -> flags_state * regs_state * callstack * memory -> Prop :=
 
   | step_Div_no_overflow:
     forall (arg_op1:in_any) (arg_op2:in_reg) (arg_out1:out_any) (arg_out2:out_reg)
       (any_tag1 any_tag2: bool)
       (mod_swap: mod_swap) (mod_flags: mod_set_flags)
       (x y:Z)
-      new_regs new_xstack new_pages new_flags
+      new_regs new_xstack new_memory new_flags
       (quot rem: Z),
       
-      fetch_apply22_swap mod_swap (regs,xstack,pgs)
+      fetch_apply22_swap mod_swap (mk_exec_state flags regs pgs xstack)
         arg_op1 arg_op2 arg_out1 arg_out2
 
         (mk_pv any_tag1 x) (mk_pv any_tag2 y) (IntValue quot, IntValue rem)
-        
-        (new_regs, new_xstack, new_pages) ->
+        (mk_exec_state flags new_regs new_memory new_xstack) ->
       y <> 0 ->
       quot = Z.div x y ->
       rem = Z.rem x y ->
@@ -34,27 +33,27 @@ Section Def.
       new_flags = apply_set_flags mod_flags flags (bflags false new_EQ new_GT) ->
       
       step_div (OpDiv arg_op1 arg_op2 arg_out1 arg_out2 mod_swap mod_flags)
-        (new_flags, new_regs, new_xstack, new_pages)
+        (new_flags, new_regs, new_xstack, new_memory)
         
   | step_Div_overflow:
     forall (arg_op1:in_any) (arg_op2:in_reg) (arg_out1:out_any) (arg_out2:out_reg)
       (any_tag1 any_tag2: bool)
       (mod_swap: mod_swap) (mod_flags: mod_set_flags)
       (x y:Z)
-      new_regs new_xstack new_pages new_flags
+      new_regs new_xstack new_memory new_flags
       (quot rem: Z),
       
-      fetch_apply22_swap mod_swap (regs,xstack,pgs)
+      fetch_apply22_swap mod_swap (mk_exec_state flags regs pgs xstack)
         arg_op1 arg_op2 arg_out1 arg_out2
 
         (mk_pv any_tag1 x) (mk_pv any_tag2 0) (IntValue 0, IntValue 0)
         
-        (new_regs, new_xstack, new_pages) ->
+        (mk_exec_state flags new_regs new_memory new_xstack) ->
 
       new_flags = apply_set_flags mod_flags flags (bflags true false false) ->
       
       step_div (OpDiv arg_op1 arg_op2 arg_out1 arg_out2 mod_swap mod_flags)
-        (new_flags, new_regs, new_xstack, new_pages).
+        (new_flags, new_regs, new_xstack, new_memory).
 
 
 
@@ -64,28 +63,21 @@ End Def.
 
 Inductive step: instruction -> smallstep :=
 | step_Div:
-  forall flags regs xstack pages ins new_flags new_regs new_xstack new_pages context_u128 gs,
-    step_div flags regs xstack pages ins (new_flags, new_regs, new_xstack, new_pages) ->
-    step ins
+  forall flags regs xstack memory ins new_flags new_regs new_xstack new_memory s1 s2,
+    step_div flags regs xstack memory ins (new_flags, new_regs, new_xstack, new_memory) ->
+    step_xstate
          {|
            gs_flags        := flags;
            gs_regs         := regs;
            gs_callstack    := xstack;
-           gs_pages        := pages;
+           gs_pages        := memory;
 
-
-           gs_context_u128 := context_u128;
-           gs_global       := gs;
          |}
          {|
            gs_flags        := new_flags;
            gs_regs         := new_regs;
            gs_callstack    := new_xstack;
-           gs_pages        := new_pages;
-
-
-           gs_context_u128 := context_u128;
-           gs_global       := gs;
-         |}
-.
+           gs_pages        := new_memory;
+         |} s1 s2 ->
+    step ins s1 s2.
 
