src/sem/LogVariants.v
@@ -17,35 +17,30 @@ Definition current_storage_fqa (xstack:callstack) : fqa_storage :=
 Inductive step: instruction -> smallstep :=
 
 | step_SLoad:
-  forall gs flags pages xstack context_u128 regs (arg_key: in_reg) (arg_dest_value: out_reg)
-    new_regs new_pages read_value key,
+  forall flags pages xstack regs (arg_key: in_reg) (arg_dest_value: out_reg)
+    new_regs new_pages read_value key (s1 s2:state),
     resolve_load_word xstack (regs,pages) arg_key key ->
 
     let fqa_storage := mk_fqa_key (current_storage_fqa xstack) key in
      
-    storage_read gs.(gs_revertable).(gs_depot) fqa_storage read_value ->
+    storage_read (gs_revertable s1).(gs_depot) fqa_storage read_value ->
     resolve_store xstack (regs, pages) arg_dest_value (IntValue read_value) (new_regs, new_pages) ->
-    step (OpSLoad arg_key arg_dest_value)
-         {|
+    step_xstate
+      {|
            gs_regs         := regs;
            gs_pages        := pages;
            gs_callstack    := xstack;
            gs_flags        := flags;
-           
-           gs_context_u128 := context_u128;
-           gs_global       := gs;
          |}
          {|
            gs_regs         := new_regs;
            gs_pages        := new_pages;
 
-
            gs_callstack    := xstack;
            gs_flags        := flags;
            
-           gs_context_u128 := context_u128;
-           gs_global       := gs;
-         |}
+         |} s1 s2 ->
+    step (OpSLoad arg_key arg_dest_value) s1 s2
 
 | step_SStore:
   forall flags pages xstack context_u128 regs (arg_key: in_reg) (arg_dest_value: out_reg)
@@ -65,23 +60,26 @@ Inductive step: instruction -> smallstep :=
     
     step (OpSLoad arg_key arg_dest_value)
          {|
+           gs_xstate := {|
            gs_regs         := regs;
            gs_pages        := pages;
-           gs_global       := gs;
            gs_callstack    := xstack;
+           gs_flags        := flags;
+                       |};
+           gs_global       := gs;
 
            
-           gs_flags        := flags;
            gs_context_u128 := context_u128;
          |}
          {|
-           gs_regs         := new_regs;
-           gs_pages        := new_pages;
+           gs_xstate := {|
+                         gs_regs         := new_regs;
+                         gs_pages        := new_pages;
+                         gs_callstack    := new_xstack;
+                         gs_flags        := flags;
+                       |};
            gs_global       := new_gs;
-           gs_callstack    := new_xstack;
 
-
-           gs_flags        := flags;
            gs_context_u128 := context_u128;
          |}
 
@@ -107,22 +105,27 @@ Inductive step: instruction -> smallstep :=
     
     step (OpToL1Message arg_key arg_value is_first)
          {|
-           gs_regs         := regs;
-           gs_pages        := pages;
-           gs_global       := gs;
-           gs_callstack    := xstack;
+           gs_xstate := {|
+                         gs_regs         := regs;
+                         gs_pages        := pages;
+                         gs_callstack    := xstack;
+
+                         gs_flags        := flags;
+                         |};
            
-           gs_flags        := flags;
+           gs_global       := gs;
            gs_context_u128 := context_u128;
          |}
          {|
-           gs_regs         := new_regs;
-           gs_pages        := new_pages;
+           gs_xstate := {|
+                         gs_regs         := new_regs;
+                         gs_pages        := new_pages;
+                         gs_callstack    := new_xstack;
+
+                         gs_flags        := flags;
+                       |};
+           
            gs_global       := new_gs;
-           gs_callstack    := new_xstack;
-
-
-           gs_flags        := flags;
            gs_context_u128 := context_u128;
          |}
          
@@ -146,23 +149,168 @@ Inductive step: instruction -> smallstep :=
     
     step (OpEvent arg_key arg_value is_first)
          {|
-           gs_regs         := regs;
-           gs_pages        := pages;
+           gs_xstate := {|
+                         gs_regs         := regs;
+                         gs_pages        := pages;
+                         gs_callstack    := xstack;
+                         gs_flags        := flags;
+                         
+                       |};
            gs_global       := gs;
-           gs_callstack    := xstack;
-           gs_flags        := flags;
+
            gs_context_u128 := context_u128;
          |}
          {|
-           gs_regs         := new_regs;
-           gs_pages        := new_pages;
+           gs_xstate := {|
+                         gs_regs         := new_regs;
+                         gs_pages        := new_pages;
+                         
+                         gs_callstack    := xstack;
+                         gs_flags        := flags;
+                       |};
+           
            gs_global       := new_gs;
 
 
-           gs_callstack    := xstack;
-           gs_flags        := flags;
            gs_context_u128 := context_u128;
          |}
 
 .
 
+(* (* FIX: if not affordable then write 0 *) *)
+(* | step_PrecompileCall: *)
+(*   forall flags pages xstack context_u128 regs (arg_params arg_extra_ergs: in_reg) (arg_dest: out_reg) is_first *)
+(*     new_regs new_pages params extra_ergs value gs new_gs, *)
+    
+(*     resolve_load_words xstack (regs, pages) [ *)
+(*         (InReg arg_params, params); *)
+(*         (InReg arg_extra_ergs, extra_ergs) *)
+(*       ] -> *)
+
+(*     PrecompileParameters.ABI.(decode)  *)
+(*    emit_event (PrecompileQuery {| *)
+(*                    ev_shard_id := current_shard xstack; *)
+(*                    ev_is_first := is_first; *)
+(*                    ev_tx_number_in_block := gs_tx_number_in_block gs; *)
+(*                    ev_address := current_contract xstack; *)
+(*                    ev_key := key; *)
+(*                    ev_value := value; *)
+(*                  |}) gs new_gs -> *)
+
+   
+   
+(*     pay (extra_ergs ) xstack new_xstack-> *)
+(*     step (OpPrecompileCall arg_key arg_extra_ergs arg_dest) *)
+(*          {| *)
+(*            gs_regs         := regs; *)
+(*            gs_pages        := pages; *)
+(*            gs_global       := gs; *)
+(*            gs_callstack    := xstack; *)
+(*            gs_flags        := flags; *)
+(*            gs_context_u128 := context_u128; *)
+(*          |} *)
+(*          {| *)
+(*            gs_regs         := new_regs; *)
+(*            gs_pages        := new_pages; *)
+(*            gs_global       := new_gs; *)
+
+
+(*            gs_callstack    := xstack; *)
+(*            gs_flags        := flags; *)
+(*            gs_context_u128 := context_u128; *)
+(*          |} *)
+         
+
+(* . *)
+
+(* (*      | OpPrecompileCall _ _ => *) *)
+(*  (* // add extra information about precompile abi in the "key" field *)
+
+(*                 if not_enough_power { *)
+(*                     // we have to update register *)
+(*                     vm_state.perform_dst0_update( *)
+(*                         vm_state.local_state.monotonic_cycle_counter, *)
+(*                         PrimitiveValue::empty(), *)
+(*                         dst0_mem_location, *)
+(*                         &self, *)
+(*                     ); *)
+(*                     return; *)
+(*                 } *)
+
+(*                 let precompile_abi = PrecompileCallABI::from_u256(src0); *)
+(*                 let PrecompileCallABI { *)
+(*                     input_memory_offset, *)
+(*                     input_memory_length, *)
+(*                     output_memory_offset, *)
+(*                     output_memory_length, *)
+(*                     per_precompile_interpreted, *)
+(*                 } = precompile_abi; *)
+
+(*                 // normal execution *)
+(*                 vm_state *)
+(*                     .local_state *)
+(*                     .callstack *)
+(*                     .get_current_stack_mut() *)
+(*                     .ergs_remaining = ergs_remaining; *)
+(*                 let memory_page_to_read = CallStackEntry::<N, E>::heap_page_from_base( *)
+(*                     vm_state *)
+(*                         .local_state *)
+(*                         .callstack *)
+(*                         .get_current_stack() *)
+(*                         .base_memory_page, *)
+(*                 ); *)
+(*                 let memory_page_to_write = CallStackEntry::<N, E>::heap_page_from_base( *)
+(*                     vm_state *)
+(*                         .local_state *)
+(*                         .callstack *)
+(*                         .get_current_stack() *)
+(*                         .base_memory_page, *)
+(*                 ); *)
+
+(*                 let timestamp_to_read = vm_state.timestamp_for_first_decommit_or_precompile_read(); *)
+(*                 let timestamp_to_write = *)
+(*                     vm_state.timestamp_for_second_decommit_or_precompile_write(); *)
+(*                 assert!(timestamp_to_read.0 + 1 == timestamp_to_write.0); *)
+
+(*                 let precompile_inner_abi = PrecompileCallInnerABI { *)
+(*                     input_memory_offset, *)
+(*                     input_memory_length, *)
+(*                     output_memory_offset, *)
+(*                     output_memory_length, *)
+(*                     memory_page_to_read: memory_page_to_read.0, *)
+(*                     memory_page_to_write: memory_page_to_write.0, *)
+(*                     precompile_interpreted_data: per_precompile_interpreted, *)
+(*                 }; *)
+(*                 let precompile_inner_abi = precompile_inner_abi.to_u256(); *)
+
+(*                 let query = LogQuery { *)
+(*                     timestamp: timestamp_for_log, *)
+(*                     tx_number_in_block, *)
+(*                     aux_byte: PRECOMPILE_AUX_BYTE, *)
+(*                     shard_id, *)
+(*                     address, *)
+(*                     key: precompile_inner_abi, *)
+(*                     read_value: U256::zero(), *)
+(*                     written_value: U256::zero(), *)
+(*                     rw_flag: false, *)
+(*                     rollback: false, *)
+(*                     is_service: is_first_message, *)
+(*                 }; *)
+(*                 vm_state.call_precompile(vm_state.local_state.monotonic_cycle_counter, query); *)
+(*                 vm_state.witness_tracer.add_sponge_marker( *)
+(*                     vm_state.local_state.monotonic_cycle_counter, *)
+(*                     SpongeExecutionMarker::StorageLogReadOnly, *)
+(*                     1..4, *)
+(*                     false, *)
+(*                 ); *)
+(*                 let result = PrimitiveValue { *)
+(*                     value: U256::from(1u64), *)
+(*                     is_pointer: false, *)
+(*                 }; *)
+(*                 vm_state.perform_dst0_update( *)
+(*                     vm_state.local_state.monotonic_cycle_counter, *)
+(*                     result, *)
+(*                     dst0_mem_location, *)
+(*                     &self, *)
+(*                 ); *)
+(* *) *)
