src/sem/Mul.v
@@ -9,12 +9,12 @@ Local Coercion u256_of : Z >-> int_mod.
 Inductive step: instruction -> smallstep :=
 
   | step_Mul:
-    forall gs flags pages xstack context_u128 regs (arg_op1:in_any) (arg_op2:in_reg) (arg_out1:out_any) (arg_out2:out_reg) any_tag1 any_tag2 mod_swap mod_flags (x y prod_hi prod_low:Z) new_regs new_xstack new_pages new_flags,
-      fetch_apply22_swap mod_swap (regs,xstack,pages)
+    forall flags pages xstack regs (arg_op1:in_any) (arg_op2:in_reg) (arg_out1:out_any) (arg_out2:out_reg) any_tag1 any_tag2 mod_swap mod_flags (x y prod_hi prod_low:Z) new_regs new_xstack new_pages new_flags s1 s2,
+      fetch_apply22_swap mod_swap (mk_exec_state flags regs pages xstack)
                      arg_op1 arg_op2
                      arg_out1 arg_out2
                      (mk_pv any_tag1 x) (mk_pv any_tag2 y) (IntValue prod_hi, IntValue prod_low)
-                     (new_regs, new_xstack, new_pages) ->
+                     (mk_exec_state flags new_regs new_pages new_xstack) ->
 
       extract_digits (x * y) word_bits 2 = [ prod_hi;  prod_low ] -> 
 
@@ -22,26 +22,19 @@ Inductive step: instruction -> smallstep :=
       let new_OF := prod_hi != zero256 in
       let new_GT := andb (negb new_OF) (negb new_EQ) in 
       new_flags = apply_set_flags mod_flags flags (bflags new_OF new_EQ new_GT) ->
-                       
-      step (OpMul arg_op1 arg_op2 arg_out1 arg_out2 mod_swap mod_flags)
+
+      step_xstate
         {|
           gs_flags        := flags;
           gs_regs         := regs;
           gs_callstack    := xstack;
           gs_pages        := pages;
-
-
-          gs_context_u128 := context_u128;
-          gs_global       := gs;
         |}
         {|
           gs_flags        := new_flags;
           gs_regs         := new_regs;
           gs_callstack    := new_xstack;
           gs_pages        := new_pages;
-
-
-          gs_context_u128 := context_u128;
-          gs_global       := gs;
-        |}
+        |} s1 s2 ->
+      step (OpMul arg_op1 arg_op2 arg_out1 arg_out2 mod_swap mod_flags) s1 s2
 .
