src/sem/UMA.v
@@ -13,13 +13,13 @@ Import Addressing.Coercions.
 
 Section Defs.
   
-  Context (old_regs: regs_state) (old_xstack: callstack) (old_pages:pages).
+  Context (old_regs: regs_state) (old_xstack: callstack) (old_pages:memory).
   Let fetch := resolve_load old_xstack (old_regs, old_pages).
-  Let fetch_word := resolve_load_word old_xstack (old_regs, old_pages).
+  Let fetch_word := resolve_load_word old_xstack (old_regs,old_pages).
   Let stores := resolve_stores old_xstack (old_regs,old_pages).
   
   Inductive step_load : instruction -> 
-                        regs_state * callstack * pages -> Prop :=
+                        regs_state * callstack * memory-> Prop :=
   | step_Load:
     forall new_xstack heap_variant enc_ptr (arg_dest:out_reg) (arg_enc_ptr:in_regimm) result new_regs new_pages selected_page in_ptr query,
       fetch_word arg_enc_ptr enc_ptr ->
@@ -75,7 +75,7 @@ Section Defs.
 
   
   Inductive step_load_ptr : instruction -> 
-                            regs_state * pages -> Prop :=
+                            regs_state * memory -> Prop :=
   | step_LoadPointerInc:
     forall enc_ptr (arg_dest arg_modptr:out_reg) (arg_enc_ptr:in_reg) result new_regs new_pages addr selected_page in_ptr out_ptr slice,
 
@@ -120,7 +120,7 @@ Section Defs.
       step_load_ptr (OpLoadPointer arg_enc_ptr arg_dest) (new_regs, new_pages)
   .
 
-  Inductive step_store: instruction -> regs_state * callstack * pages -> Prop :=
+  Inductive step_store: instruction -> regs_state * callstack * memory -> Prop :=
 
   | step_StoreInc:
     forall new_xstack heap_variant enc_ptr (arg_modptr:out_reg) (arg_enc_ptr:in_regimm) (arg_val:in_reg) value new_regs new_pages selected_page in_ptr ptr_incremented pages1 query modified_page,
@@ -190,78 +190,67 @@ End Defs.
 Inductive step  : instruction -> smallstep := 
 
 | step_LoadVariant:
-  forall gs flags  pages xstack new_xstack context_u128 regs new_regs new_pages ins,
+  forall flags  pages xstack new_xstack regs new_regs new_pages ins s1 s2,
     step_load regs xstack pages ins (new_regs, new_xstack, new_pages) ->
-    step ins 
-         {|
-           gs_regs         := regs;
-           gs_callstack    := xstack;
-           gs_pages        := pages;
+    step_xstate
+      {|
+        gs_regs         := regs;
+        gs_callstack    := xstack;
+        gs_pages        := pages;
 
-
-           gs_flags        := flags;
-           gs_context_u128 := context_u128;
-           gs_global       := gs;
-         |}
-         {|
-           gs_regs         := new_regs;
-           gs_callstack    := new_xstack;
-           gs_pages        := new_pages;
-
-
-           gs_flags        := flags;
-           gs_context_u128 := context_u128;
-           gs_global       := gs;
-         |}
+        gs_flags        := flags;
+      |}
+      {|
+        gs_regs         := new_regs;
+        gs_callstack    := new_xstack;
+        gs_pages        := new_pages;
+        
+        
+        gs_flags        := flags;
+      |} s1 s2 ->
+    step ins s1 s2
 | step_StoreVariant:
-  forall gs flags  pages xstack new_xstack context_u128 regs new_regs new_pages ins,
+  forall flags  pages xstack new_xstack regs new_regs new_pages ins s1 s2,
     step_store regs xstack pages ins (new_regs, new_xstack, new_pages) ->
-    step ins 
-         {|
-           gs_regs         := regs;
-           gs_callstack    := xstack;
-           gs_pages        := pages;
 
+    step_xstate
+      {|
+        gs_regs         := regs;
+        gs_callstack    := xstack;
+        gs_pages        := pages;
 
-           gs_flags        := flags;
-           gs_context_u128 := context_u128;
-           gs_global       := gs;
-         |}
-         {|
-           gs_regs         := new_regs;
-           gs_callstack    := new_xstack;
-           gs_pages        := new_pages;
-
-
-           gs_flags        := flags;
-           gs_context_u128 := context_u128;
-           gs_global       := gs;
-         |}
+        gs_flags        := flags;
+      |}
+      {|
+        gs_regs         := new_regs;
+        gs_callstack    := new_xstack;
+        gs_pages        := new_pages;
+        
+        
+        gs_flags        := flags;
+      |} s1 s2 ->
+    step ins s1 s2
+    
 | step_LoadPtrVariant:
-  forall gs flags  pages xstack context_u128 regs new_regs new_pages ins,
+  forall flags  pages xstack regs new_regs new_pages ins s1 s2,
     step_load_ptr regs xstack pages ins (new_regs, new_pages) ->
-    step ins 
-         {|
-           gs_regs         := regs;
-           gs_callstack    := xstack;
-           gs_pages        := pages;
+    step_xstate
+      {|
+        gs_regs         := regs;
+        gs_pages        := pages;
 
+        gs_callstack    := xstack;
+        gs_flags        := flags;
+      |}
+      {|
+        gs_regs         := new_regs;
+        gs_pages        := new_pages;
 
-           gs_flags        := flags;
-           gs_context_u128 := context_u128;
-           gs_global       := gs;
-         |}
-         {|
-           gs_regs         := new_regs;
-           gs_pages        := new_pages;
-
-
-           gs_callstack    := xstack;
-           gs_flags        := flags;
-           gs_context_u128 := context_u128;
-           gs_global       := gs;
-         |}
-.
+        
+        gs_callstack    := xstack;
+        gs_flags        := flags;
+      |} s1 s2 ->
+    step ins s1 s2 .
 
 (** If set to [Inc32], the instruction:
 
